theories/Projection.v
@@ -1,0 +1,12 @@
+From mathcomp.ssreflect Require Import all_ssreflect.
+
+Set Implicit Arguments.
+Unset Strict Implicit.
+Import Prenex Implicits.
+
+Require Export MPST.Projection.IProject.
+Require Export MPST.Projection.CProject.
+Require Export MPST.Projection.QProject.
+Require Export MPST.Projection.Correctness.
+
+Definition Projection G P := eProject G P.1 /\ qProject G P.2.
