theories/Projection/QProject.v
@@ -1,0 +1,111 @@
+From mathcomp.ssreflect Require Import all_ssreflect seq.
+From mathcomp Require Import finmap.
+Set Implicit Arguments.
+Unset Strict Implicit.
+Import Prenex Implicits.
+
+From Paco Require Import paco paco2.
+
+Require Import MPST.Common.
+Require Import MPST.Global.
+Require Import MPST.Local.
+
+Open Scope fmap.
+
+Definition qproj_rel := ig_ty -> {fmap role * role -> seq (lbl * mty) } -> Prop.
+Inductive qProject : qproj_rel :=
+| qprj_end G : qProject (ig_end G) [fmap]%fmap
+
+| qprj_none p p' CONT Q :
+    (forall l Ty G, CONT l = Some (Ty, G) -> qProject G Q) ->
+    Q.[? (p,p')] = None ->
+    qProject (ig_msg None p p' CONT) Q
+
+| qprj_some p p' CONT l Ty G Q Q':
+    CONT l = Some (Ty, G) ->
+    deq Q' (p, p') == Some ((l, Ty), Q) ->
+    qProject G Q ->
+    qProject (ig_msg (Some l) p p' CONT) Q'
+.
+Hint Constructors qProject.
+
+Lemma qProject_end_inv_aux Q iG G:
+  qProject iG Q ->  iG = (ig_end G) ->
+  Q = ([fmap]%fmap).
+Proof.
+  case =>//=.
+Qed.
+
+Lemma qProject_end_inv Q G:
+  qProject (ig_end G) Q ->
+  Q = ([fmap]%fmap).
+Proof.
+    by move=> hp; apply: (@qProject_end_inv_aux Q _ G hp).
+Qed.
+
+Lemma qProject_None_inv_aux F T C Q GG:
+  qProject GG Q ->
+  GG = (ig_msg None F T C) ->
+  Q.[? (F,T)] = None /\ forall l Ty G,
+      (C l = Some (Ty, G) -> qProject G Q).
+Proof.
+  case =>//=.
+  move=> p p' CONT Q0 IH neq [eq1 eq2 eq3].
+  split; [by rewrite -eq1 -eq2| rewrite -eq3].
+    by apply IH.
+Qed.
+
+Lemma qProject_None_inv F T C Q :
+  qProject (ig_msg None F T C) Q ->
+  Q.[? (F,T)] = None /\ forall l Ty G,
+      (C l = Some (Ty, G) -> qProject G Q).
+Proof.
+    by move=> hp; move: (@ qProject_None_inv_aux F T C _ _ hp)=>H; apply/H.
+Qed.
+
+Lemma qProject_Some_inv_aux l F T C Q GG:
+  qProject GG Q ->
+  GG = (ig_msg (Some l) F T C) ->
+  (exists Ty G Q',
+      C l = Some (Ty, G) /\
+      deq Q (F, T) == Some ((l, Ty), Q') /\
+      qProject G Q').
+Proof.
+  case =>//.
+  move=> p p' CONT l0 Ty G Q0 Q' CONTL0 deqQ' qpro [eq1 eq2 eq3 eq4].
+  rewrite -eq1 -eq2 -eq3 -eq4;  exists Ty, G, Q0.
+  by split; [| split; [|]].
+Qed.
+
+Lemma qProject_Some_inv l F T C Q:
+  qProject (ig_msg (Some l) F T C) Q ->
+  exists Ty G Q', C l = Some (Ty, G) /\
+                  deq Q (F, T) == Some ((l, Ty), Q') /\
+                  qProject G Q'.
+Proof.
+  move=> hp; move: (@qProject_Some_inv_aux l F T C Q _ hp).
+  by move=> triv; apply triv.
+Qed.
+
+Lemma deq_elsewhere Q Q' k0 k L Ty:
+  deq Q' k0 == Some (L, Ty, Q) -> k != k0 ->
+  Q'.[?k]=Q.[?k].
+Proof.
+  rewrite /deq; case E: (Q'.[? k0]) =>[qs|] //=; case qs => [|q qs0] //=.
+  case: ifP; move=> _; rewrite -(rwP eqP); move=> [_ <-].
+  + by rewrite fnd_rem1; case: ifP.
+  + by rewrite fnd_set; case: ifP.
+Qed.
+
+Lemma deq_singleton (Q:{fmap role * role -> seq (lbl * mty) }) p q v:
+  Q.[?(p,q)] == None ->
+  deq Q.[(p, q) <- [:: v]] (p, q) = Some (v, Q).
+Proof.
+  move=> Qnone; rewrite /deq fnd_set; case: ifP; rewrite eq_refl //=; elim.
+  apply: f_equal; apply: injective_projections =>//=.
+  rewrite -fmapP; move=> pq; rewrite fnd_rem1; case: ifP.
+  + move=> neq; rewrite fnd_set; case: ifP =>//=.
+    by rewrite (negbTE neq) //=.
+  + move=> eq; move: (negbNE (negbT eq)).
+    by rewrite -(rwP eqP) =>->; rewrite (rwP eqP) eq_sym.
+Qed.
